lib/fst/Lib.Buffer.fst
@@ -21,8 +21,12 @@ friend Lib.Sequence
 
 let length #a b = B.length b
 
+let as_seq_gsub #a #len h b start n = ()
+
 let sub #a #len #olen b start n =
   B.sub b (size_to_UInt32 start) (size_to_UInt32 n)
+
+let as_seq_igsub #a #len h b start n = ()
 
 let isub #a #len #olen b start n =
   IB.isub b (size_to_UInt32 start) (size_to_UInt32 n)
